A big crunch

nsl/Games.ec
@@ -876,1309 +876,306 @@ qed.
 (* ------------------------------------------------------------------------------------------ *)
 (* Game 8 invariants *)
 
-(* Return the messages from a state *)
-op get_msgs s : ctxt list =
-with s = Accepted t _   => [t.`1.`2; t.`2; t.`3]
-with s = Observed t _   => [t.`1.`2; t.`2; t.`3]
-with s = IPending _ m1   => [m1.`2]
-with s = RPending _ m1 m2 => [m1.`2; m2]
-with s = Aborted v  =>
-  match v with
-  | R1 => []
-  | I m1 => [m1]
-  | R2 m1 m2 => [m1; m2]
-end.
+(* Return the first sent message from a state *)
+op fst_msg s : ctxt option =
+with s = IPending _ m1   => Some m1.`2
+with s = RPending _ m1 m2 => Some m1.`2
+with s = Accepted t _   => Some t.`1.`2
+with s = Observed t _   => Some t.`1.`2
+with s = Aborted v  => None.
 
-inductive Game8_inv
-  (sm: (id * int, role * instance_state) fmap)
-  (skm : (trace, skey) fmap)
-  (dm : ((id * id) * msg_data * ctxt, nonce) fmap)
-  (a: id) (i: int)
-=
-| Game8_undef of
-    (sm.[a, i] = None)
-| Game8_aborted_r1 of
-    (sm.[a, i] = Some (Responder, Aborted R1))
-| Game8_aborted_i b c1 of
-    (sm.[a, i] = Some (Initiator, Aborted (I c1)))
-  & (((a, b), msg1_data a b, c1) \in dm)
-| Game8_aborted_r2 b c1 c2 of
-    (sm.[a, i] = Some (Responder, Aborted (R2 c1 c2)))
-  & (((b, a), msg2_data b a c1, c2) \in dm)
-| Game8_ipending b c1 of
-    (sm.[a, i] = Some (Initiator, IPending (b, witness, witness, c1) (a, c1)))
-  & (((a, b), msg1_data a b, c1) \in dm)
-  & (forall c2 c3, ((a, b), msg3_data a b c1 c2, c3) \notin dm)
-| Game8_rpending b c1 c2 of
-    (sm.[a, i] = Some (Responder, RPending (b, witness, witness, witness, c1, c2) (b, c1) c2))
-  & (((b, a), msg2_data b a c1, c2) \in dm)
-| Game8_accepted_i b j st c1 c2 c3 of
-    (sm.[a, i] = Some (Initiator, Accepted ((a, c1), c2, c3) witness))
-  & (((a, b), msg3_data a b c1 c2, c3) \in dm)
-  & (sm.[b, j] = Some (Responder, st))
-  & (c1 \in get_msgs st /\ c2 \in get_msgs st)
-  & (c3 \in get_msgs st <=> get_trace st <> None)
-  & (!is_observed st => ((a, c1), c2, c3) \notin skm)
-| Game8_accepted_r b j st c1 c2 c3 of
-    (sm.[a, i] = Some (Responder, Accepted ((b, c1), c2, c3) witness))
-  & (((b, a), msg3_data b a c1 c2, c3) \in dm)
-  & (sm.[b, j] = Some (Initiator, st))
-  & (get_trace st = Some ((b, c1), c2, c3))
-  & (!is_observed st => ((b, c1), c2, c3) \notin skm)
-| Game8_observed r id1 id2 c1 c2 c3 k of
-    (sm.[a, i] = Some (r, Observed ((id1, c1), c2, c3) k))
-  & (((id1, id2), msg3_data id1 id2 c1 c2, c3) \in dm)
-  & (((id1, c1), c2, c3) \in skm)
-  & (a = id1 \/ a = id2).
+(* Return the second sent message from a state *)
+op snd_msg s : ctxt option =
+with s = IPending _ m1   => None
+with s = RPending _ m1 m2 => Some m2
+with s = Accepted t _   => Some t.`2
+with s = Observed t _   => Some t.`2
+with s = Aborted v  => None.
 
-inductive Game8_inv_dm
-  (sm: (id * int, role * instance_state) fmap)
-  (dm : ((id * id) * msg_data * ctxt, nonce) fmap)
-  (c : ctxt)
-=
-| Game8_dm_undef of
-    (forall a b, ((a, b), msg1_data a b, c) \notin dm)
-  & (forall a b c1, ((a, b), msg2_data a b c1, c) \notin dm)
-  & (forall a b c1 c2, ((a, b), msg3_data a b c1 c2, c) \notin dm)
-| Game8_dm_m1 a b i st of
-    (((a, b), msg1_data a b, c) \in dm)
-  & (sm.[a, i] = Some (Initiator, st))
-  & (c \in get_msgs st)
-  & (forall h st',
-       sm.[h] = Some (Initiator, st') =>
-       c \in get_msgs st' =>
-       h = (a, i))
-| Game8_dm_m2 a b j st c1 of
-    (((a, b), msg1_data a b, c1) \in dm)
-  & (((a, b), msg2_data a b c1, c) \in dm)
-  & (sm.[b, j] = Some (Responder, st))
-  & (c1 \in get_msgs st)
-  & (c \in get_msgs st)
-  & (forall h st',
-       sm.[h] = Some (Responder, st') =>
-       c1 \in get_msgs st' =>
-       c \in get_msgs st' =>
-       h = (b, j))
-| Game8_dm_m3 a b i st c1 c2 of
-    (((a, b), msg1_data a b, c1) \in dm)
-  & (((a, b), msg2_data a b c1, c2) \in dm)
-  & (((a, b), msg3_data a b c1 c2, c) \in dm)
-  & (sm.[a, i] = Some (Initiator, st))
-  & (c1 \in get_msgs st)
-  & (c2 \in get_msgs st)
-  & (c \in get_msgs st)
-  & (forall h st',
-       sm.[h] = Some (Initiator, st') =>
-       c1 \in get_msgs st' =>
-       c2 \in get_msgs st' =>
-       c \in get_msgs st' =>
-       h = (a, i))
-.
-
-op Game8_inv_full
+op Game8_inv
   (sm: (id * int, role * instance_state) fmap)
   (dm : ((id * id) * msg_data * ctxt, nonce) fmap)
   (skm : (trace, skey) fmap)
 =
-  (forall a i, Game8_inv sm skm dm a i)
-  /\ (forall c, Game8_inv_dm sm dm c)
-  /\ (forall pk ad pk' ad' c,
-        (pk, ad, c) \in dm =>
-        (pk', ad', c) \in dm =>
-        (pk, ad) = (pk', ad'))
-  /\ (forall a c1 c2 c3, ((a, c1), c2, c3) \in skm => exists b, ((a, b), msg3_data a b c1 c2, c3) \in dm).
+(* Unicity of pending initiators *)
+   (forall h h' c r b psk na m1 st',
+    sm.[h] = Some (r, IPending (b, psk, na, c) m1)
+    /\ sm.[h'] = Some (r, st')
+    /\ fst_msg st' = Some c
+    => h = h')
+
+(* Unicity of pending responders *)
+/\ (forall h h' c1 c r b psk na nb m1 m2 st',
+    sm.[h] = Some (r, RPending (b, psk, na, nb, c1, c) m1 m2)
+    /\ sm.[h'] = Some (r, st')
+    /\ snd_msg st' = Some c
+    => h = h')
+
+(* Unicity of completed sessions with same trace and role *)
+/\ (forall t h h' r s s',
+    sm.[h] = Some (r, s) /\ sm.[h'] = Some (r, s')
+    /\ get_trace s = Some t /\ get_trace s' = Some t
+    => h = h' /\ s = s')
+
+(* Session state and log relationships *)
+/\ (forall a i r b psk na c1 m1,
+      sm.[a, i] = Some (r, IPending (b, psk, na, c1) m1)
+      => ((a, b), msg1_data a b, c1) \in dm /\ r = Initiator /\ m1 = (a, c1))
+
+/\ (forall a i r b psk na nb c1 c2 m1 m2,
+      sm.[a, i] = Some (r, RPending (b, psk, na, nb, c1, c2) m1 m2)
+      => ((b, a), msg1_data b a, c1) \in dm /\ ((b, a), msg2_data b a c1, c2) \in dm
+      /\ r = Responder /\ m1 = (b, c1) /\ c2 = m2)
+
+/\ (forall a i r b m1 m2 m3 sk,
+      sm.[a, i] = Some (r, Accepted ((b, m1), m2, m3) sk)
+      => (exists pk ad, (pk, ad, m1) \in dm) /\ (exists pk ad, (pk, ad, m2) \in dm))
+
+/\ (forall a i r b m1 m2 m3 sk,
+      sm.[a, i] = Some (r, Observed ((b, m1), m2, m3) sk)
+      => (exists pk ad, (pk, ad, m1) \in dm) /\ (exists pk ad, (pk, ad, m2) \in dm))
+
+(* SK implies existence of an observed session *)
+/\ (forall t, t \in skm => exists a i r k, sm.[a, i] = Some (r, Observed t k)).
 
 hoare Game8_inv_send_msg1: Game8.send_msg1:
-  Game8_inv_full Game8.state_map Game8.dec_map Game8.sk_map
+  Game8_inv Game8.state_map Game8.dec_map Game8.sk_map
   ==>
-  Game8_inv_full Game8.state_map Game8.dec_map Game8.sk_map.
+  Game8_inv Game8.state_map Game8.dec_map Game8.sk_map.
 proof.
 proc.
 sp; wp; if=> //.
 seq 1 : (#pre); 1: by auto.
-auto=> />.
-move=> &m inv1 inv2 inv3 inv4 ai_nin_sm ab_in_psk bad.
+auto => />.
+
+move => &m uniq_pi uniq_pr uniq_comp ss_log_ip ss_log_rp ss_log_acc ss_log_obs sk_obs sm psk bad.
 do! split.
 
-(* State Map invariant *)
-move => a' i'.
-case: ((a', i') = (a, i){m}) => /> => [| neq].
-+ apply (Game8_ipending _ _ _ _ _ b{m} ca{m}).
-  + by rewrite get_set_sameE.
-  + by rewrite mem_set.
-  move => c2 c3.
-  rewrite mem_set /=.
-  case (inv2 c3) => /#.
-
-case (inv1 a' i').
-+ move => sm.
-  apply Game8_undef.
-  by rewrite get_set_neqE.
-+ move => sm.
-  apply (Game8_aborted_r1 _ _ _ _ _).
-  by rewrite get_set_neqE.
-+ move => b' c1 sma' dm .
-  apply (Game8_aborted_i _ _ _ _ _ b' c1) => //.
-  + by rewrite get_set_neqE.
-  by rewrite mem_set; left.
-+ move => b' c1 c2 sma' dmc2.
-  apply (Game8_aborted_r2 _ _ _ _ _ b' c1 c2) => //.
-  + by rewrite get_set_neqE.
-  by rewrite mem_set; left.
-+ move => b' c1 sma' dmc1 ndmc1.
-  apply (Game8_ipending _ _ _ _ _ b' c1) => //.
-  + by rewrite get_set_neqE.
-  + by rewrite mem_set; left.
-  smt(mem_set).
-+ move => b' c1 c2 sma' dmc2.
-  apply (Game8_rpending _ _ _ _ _ b' c1 c2) => //.
-  + by rewrite get_set_neqE.
-  by rewrite mem_set; left.
-+ move => b j stb c1 c2 c3 sma' dmc3 nsk smbj c_in_stbj neqbj.
-  apply (Game8_accepted_i _ _ _ _ _ b j stb c1 c2 c3) => //.
-  + by rewrite get_set_neqE.
-  + by rewrite mem_set; left.
-  smt(get_set_neqE).
-+ move => b' j st c1 c2 c3 sma' dmc3 smbj obs_sk.
-  apply (Game8_accepted_r _ _ _ _ _ b' j st c1 c2 c3) => //.
-  + by rewrite get_set_neqE.
-  + smt(mem_set).
-  smt(get_set_neqE).
-move => r id1 id2 c1 c2 c3 k sma' dmc3 skm_k ids_eq.
-apply (Game8_observed _ _ _ _ _ r id1 id2 c1 c2 c3 k) => //.
-+ by rewrite get_set_neqE.
-by rewrite mem_set; left.
-
-(* Decmap invariant *)
-move => c.
-case (c = ca{m}) => /> => [| neq].
-+ apply (Game8_dm_m1 _ _ _ a{m} b{m} i{m} (IPending (b, witness, witness, ca){m} (a, ca){m})) => //.
-  + by rewrite mem_set; right.
-  + by rewrite get_set_sameE.
-  + move => [b' j'] st'.
-    rewrite get_setE.
-    case ((b', j') = (a, i){m}) => />.
-    move => neq smbj'.
-    case (inv1 b' j'); rewrite smbj' //=.
-    + smt().
-    + smt().
-    + move => /> b j stb c1 c2 c3.
-      case (inv2 c3); smt().
-    move => /> id1 id2 c1 c2 c3.
-    by case (inv2 c3); smt().
-
-case (inv2 c).
-+ move => ndm1 ndm2 ndm3.
-  apply (Game8_dm_undef _ _ _) => //.
-  + smt(mem_set).
-  + smt(mem_set).
-  smt(mem_set).
-
-+ move => a' b' i' st dmc smai c_in_st uniq.
-  apply (Game8_dm_m1 _ _ _ a' b' i' st) => //.
-  + smt(mem_set).
-  + smt(get_setE).
+move => h h' c r b' psk' na' m1 st'.
+rewrite !get_setE.
+case (h = (a, i){m}).
++ case (h' = (a, i){m}) => //.
   smt(get_setE).
-
-+ move => a' b' j' st c1 dmc1 dmc smbj c1_in_st c_in_st uniq.
-  apply (Game8_dm_m2 _ _ _ a' b' j' st c1) => //.
-  + smt(mem_set).
-  + smt(mem_set).
-  + smt(get_setE).
+case (h' = (a, i){m}) => //. 
++ move => />.
   smt(get_setE).
+smt().
 
-move => a' b' i' st c1 c2 dmc1 dmc2 dmc smai c1_in_st c2_in_st c_in_st uniq.
-apply (Game8_dm_m3 _ _ _ a' b' i' st c1 c2) => //.
-+ smt(mem_set).
-+ smt(mem_set).
-+ smt(mem_set).
-+ smt(get_setE).
 smt(get_setE).
-
-(* Ciphertext Decmap Uniqueness *)
-smt(mem_set).
-
-(* Secret Key Decmap *)
-smt(mem_set).
+smt(get_setE).
+smt(get_setE).
+smt(get_setE).
+smt(get_setE).
+smt(get_setE).
+smt(get_setE).
 qed.
 
+
 hoare Game8_inv_send_msg2: Game8.send_msg2:
-  Game8_inv_full Game8.state_map Game8.dec_map Game8.sk_map
+  Game8_inv Game8.state_map Game8.dec_map Game8.sk_map
   ==>
-  Game8_inv_full Game8.state_map Game8.dec_map Game8.sk_map.
+  Game8_inv Game8.state_map Game8.dec_map Game8.sk_map.
 proof.
 proc.
 sp; wp; if=> //.
 sp; match => //.
 + auto=> />.
-  move=> &m ? ? inv1 inv2 inv3 inv4 ? ?.
+  move => &m dm sm uniq_pi uniq_pr uniq_comp ss_log_ip ss_log_rp ss_log_acc ss_log_obs sk_obs smnin pskin.
   do! split.
-
-  (* State Map invariant *)
-  move=> b' j'.
-  case: ((b', j') = (b, j){m}) => /> => [|neq_bj].
-  - apply (Game8_aborted_r1 _ _ _ _ _).
-    by rewrite get_set_sameE.
-
-  case (inv1 b' j').
-  + move => sm.
-    apply Game8_undef.
-    by rewrite get_set_neqE.
-  + move => sm.
-    apply (Game8_aborted_r1 _ _ _ _ _).
-    by rewrite get_set_neqE.
-  + move => a' c1 sma' dm.
-    apply (Game8_aborted_i _ _ _ _ _ a' c1) => //.
-    by rewrite get_set_neqE.
-  + move => a' c1 c2 smb' dmc2.
-    apply (Game8_aborted_r2 _ _ _ _ _ a' c1 c2) => //.
-    by rewrite get_set_neqE.
-  + move => a' c1 smb' dmc1 ndmc1.
-    apply (Game8_ipending _ _ _ _ _ a' c1) => //.
-    by rewrite get_set_neqE.
-  + move => a' c1 c2 smb' dmc2.
-    apply (Game8_rpending _ _ _ _ _ a' c1 c2) => //.
-    by rewrite get_set_neqE.
-  + move => b j stb c1 c2 c3 sma' dmc3 nsk smbj cs_in_stb neqbj.
-    apply (Game8_accepted_i _ _ _ _ _ b j stb c1 c2 c3) => //.
-    + by rewrite get_set_neqE.
-    smt(get_set_neqE).
-  + move => a' i st c1 c2 c3 smb' dmc3 smai obs_sk.
-    apply (Game8_accepted_r _ _ _ _ _ a' i st c1 c2 c3) => //.
-    + by rewrite get_set_neqE.
-    smt(get_set_neqE).
-  move => r id1 id2 c1 c2 c3 k smb' dmc3 skm_k ids_eq.
-  apply (Game8_observed _ _ _ _ _ r id1 id2 c1 c2 c3 k) => //.
-  by rewrite get_set_neqE.
-
-  (* Decmap invariant *)
-  move => c.
-
-  case (inv2 c).
-  + move => ndm1 ndm2 ndm3.
-    exact (Game8_dm_undef _ _ _).
-
-  + move => a' b' i' st dmc smai c_in_st uniq.
-    apply (Game8_dm_m1 _ _ _ a' b' i' st) => //.
-    + smt(get_setE).
-    smt(get_setE).
-
-  + move => a' b' j' st c1 dmc1 dmc smbj c1_in_st c_in_st uniq.
-    apply (Game8_dm_m2 _ _ _ a' b' j' st c1) => //.
-    + smt(get_setE).
-    smt(get_setE).
-
-  move => a' b' i' st c1 c2 dmc1 dmc2 dmc smai c1_in_st c2_in_st c_in_st uniq.
-  apply (Game8_dm_m3 _ _ _ a' b' i' st c1 c2) => //.
-  + smt(get_setE).
+  
   smt(get_setE).
-
-  (* Ciphertext Decmap Uniqueness *)
-  exact inv3.
+  smt(get_setE).
+  smt(get_setE).
+  smt(get_setE).
+  smt(get_setE).
+  smt(get_setE).
+  smt(get_setE).
+  smt(get_setE).
 
 seq 1 : (#pre); 1: by auto.
 auto => />.
-move => &m ? ? inv1 inv2 inv3 inv4 bj_nin_sm ab_in_psk bad.
-
+move => &m dm sm uniq_pi uniq_pr uniq_comp ss_log_ip ss_log_rp ss_log_acc ss_log_obs sk_obs smnin pskin bad.
 do! split.
 
-(* State Map invariant *)
-move => b' j'.
-case: ((b', j') = (b, j){m}) => /> => [|neq_bj].
-- apply (Game8_rpending _ _ _ _ _ a{m} ca{m} cb{m}) => //.
-  + by rewrite get_set_sameE.
-  by rewrite mem_set; right.
-
-case (inv1 b' j').
-+ move => sm.
-  apply Game8_undef.
-  by rewrite get_set_neqE.
-+ move => sm.
-  apply (Game8_aborted_r1 _ _ _ _ _).
-  by rewrite get_set_neqE.
-+ move => a' c1 sma' dm.
-  apply (Game8_aborted_i _ _ _ _ _ a' c1) => //.
-  + by rewrite get_set_neqE.
-  smt(mem_set).
-+ move => a' c1 c2 smb' dmc2.
-  apply (Game8_aborted_r2 _ _ _ _ _ a' c1 c2) => //.
-  + by rewrite get_set_neqE.
-  smt(mem_set).
-+ move => a' c1 smb' dmc1 ndmc1.
-  apply (Game8_ipending _ _ _ _ _ a' c1) => //.
-  + by rewrite get_set_neqE.
-  + smt(mem_set).
-  smt(mem_set).
-+ move => a' c1 c2 smb' dmc2.
-  apply (Game8_rpending _ _ _ _ _ a' c1 c2) => //.
-  + by rewrite get_set_neqE.
-  smt(mem_set).
-+ move => b j stb c1 c2 c3 sma' dmc3 nsk smbj cs_in_stb neqbj.
-  apply (Game8_accepted_i _ _ _ _ _ b j stb c1 c2 c3) => //.
-  + by rewrite get_set_neqE.
-  + smt(mem_set).
-  smt(get_set_neqE).
-+ move => a' i st c1 c2 c3 smb' dmc3 smai obs_sk.
-  apply (Game8_accepted_r _ _ _ _ _ a' i st c1 c2 c3) => //.
-  + by rewrite get_set_neqE.
-  + smt(mem_set).
-  smt(get_set_neqE).
-move => r id1 id2 c1 c2 c3 k smb' dmc3 skm_k ids_eq.
-apply (Game8_observed _ _ _ _ _ r id1 id2 c1 c2 c3 k) => //.
-+ by rewrite get_set_neqE.
-smt(mem_set).
-
-(* Decmap invariant *)
-move => c.
-
-case (c = cb{m}) => /> => [| neq].
-+ apply (Game8_dm_m2 _ _ _ a{m} b{m} j{m} (RPending (a, witness, witness, witness, ca, cb){m} (a, ca){m} cb{m}) ca{m}) => //.
-  + smt(mem_set).
-  + by rewrite mem_set.
-  + by rewrite get_set_sameE.
-  + move => [a' i'] st'.
-    rewrite get_setE.
-    case ((a', i') = (b, j){m}) => />.
-    move => neq smai'.
-    case (inv1 a' i'); rewrite smai' //=.
-    + smt().
-    + smt().
-    + move => /> a i st c1 c2 c3.
-      case (inv2 c3); smt().
-    move => /> id1 id2 c1 c2 c3.
-    case (inv2 c3); smt().
-
-case (inv2 c).
-+ move => ndm1 ndm2 ndm3.
-  apply (Game8_dm_undef _ _ _) => //.
-  + smt(mem_set).
-  + smt(mem_set).
-  smt(mem_set).
-
-+ move => a' b' i' st dmc smai c_in_st uniq.
-  apply (Game8_dm_m1 _ _ _ a' b' i' st) => //.
-  + smt(mem_set).
-  + smt(get_setE).
-  smt(get_setE).
-
-+ move => a' b' j' st c1 dmc1 dmc smbj c1_in_st c_in_st uniq.
-  apply (Game8_dm_m2 _ _ _ a' b' j' st c1) => //.
-  + smt(mem_set).
-  + smt(mem_set).
-  + smt(get_setE).
-  smt(get_setE).
-
-move => a' b' i' st c1 c2 dmc1 dmc2 dmc smai c1_in_st c2_in_st c_in_st uniq.
-apply (Game8_dm_m3 _ _ _ a' b' i' st c1 c2) => //.
-+ smt(mem_set).
-+ smt(mem_set).
-+ smt(mem_set).
-+ smt(get_setE).
 smt(get_setE).
 
+move => h h' c1 c r b' psk' na' nb' m1' m2 st'.
+rewrite !get_setE.
+case (h = (b, j){m}).
++ case (h' = (b, j){m}) => //.
+  smt(get_setE).
+case (h' = (b, j){m}) => //. 
++ move => />.
+  smt(get_setE).
+smt().
 smt(get_setE).
-
+smt(get_setE).
+smt(get_setE).
+smt(get_setE).
+smt(get_setE).
 smt(get_setE).
 qed.
 
 hoare Game8_inv_send_msg3: Game8.send_msg3:
-  Game8_inv_full Game8.state_map Game8.dec_map Game8.sk_map
+  Game8_inv Game8.state_map Game8.dec_map Game8.sk_map
   ==>
-  Game8_inv_full Game8.state_map Game8.dec_map Game8.sk_map.
+  Game8_inv Game8.state_map Game8.dec_map Game8.sk_map.
 proof.
 proc.
 sp; wp; if=> //.
 sp; match => //.
 sp; match => //.
 + auto => />.
-  move=> &m ? ? inv1 inv2 inv3 inv4 ?.
-  have smai : Game8.state_map.[a, i]{m} = Some (role, IPending (b, psk, na, ca) m1){m} by smt().
-  case (inv1 a{m} i{m}); rewrite smai //=.
-  move => /> !->> dmca ndmca.
+  move => &m dm sm uniq_pi uniq_pr uniq_comp ss_log_ip ss_log_rp ss_log_acc ss_log_obs sk_obs smin.
   do! split.
-
-  (* State Map invariant *)
-  move => a' i'.
-  case: ((a', i') = (a, i){m}) => /> => [| neq].
-  + apply (Game8_aborted_i _ _ _ _ _ b{m} ca{m}) => //.
-    by rewrite get_set_sameE.
-
-  case (inv1 a' i').
-  + move => sm.
-    apply Game8_undef.
-    by rewrite get_set_neqE.
-  + move => sm.
-    apply (Game8_aborted_r1 _ _ _ _ _).
-    by rewrite get_set_neqE.
-  + move => b' c1 sma' dm .
-    apply (Game8_aborted_i _ _ _ _ _ b' c1) => //.
-    by rewrite get_set_neqE.
-  + move => b' c1 c2 sma' dmc2.
-    apply (Game8_aborted_r2 _ _ _ _ _ b' c1 c2) => //.
-    by rewrite get_set_neqE.
-  + move => b' c1 sma' dmc1 ndmc1.
-    apply (Game8_ipending _ _ _ _ _ b' c1) => //.
-    by rewrite get_set_neqE.
-  + move => b' c1 c2 sma' dmc2.
-    apply (Game8_rpending _ _ _ _ _ b' c1 c2) => //.
-    + by rewrite get_set_neqE.
-  + move => b' j st c1 c2 c3 sma' dmc3 nsk smbj neq_bj.
-    apply (Game8_accepted_i _ _ _ _ _ b' j st c1 c2 c3) => //.
-    + by rewrite get_set_neqE.
-    smt(get_setE).
-  + move => b' j st c1 c2 c3 sma' dmc3 smbj neq_bj.
-    apply (Game8_accepted_r _ _ _ _ _ b' j st c1 c2 c3) => //.
-    + by rewrite get_set_neqE.
-    case ((b', j) = (a, i){m}); 2: smt(get_setE).
-    move => />.
-    case (inv2 c3); 1..3: smt(get_setE).
-    smt(get_set_neqE).
-  move => r id1 id2 c1 c2 c3 k sma' dmc3 skm_k ids_eq.
-  apply (Game8_observed _ _ _ _ _ r id1 id2 c1 c2 c3 k) => //.
-  by rewrite get_set_neqE.
-
-  (* Decmap invariant *)
-  move => c.
-
-  case (inv2 c).
-  + move => ndm1 ndm2 ndm3.
-    exact (Game8_dm_undef _ _ _).
-
-  + move => a' b' i' st.
-    case ((a', i') = (a, i){m}) => /> => [| neq].
-    + rewrite smai => /> dmc uniq.
-      apply (Game8_dm_m1 _ _ _ a{m} b{m} i{m} (Aborted (I ca{m}))) => //.
-      + by rewrite get_set_sameE.
-      smt(get_setE).
-    move => dmc smai' c_in_st uniq.
-    apply (Game8_dm_m1 _ _ _ a' b' i' st) => //.
-    + smt(get_setE).
-    smt(get_setE).
-
-  + move => a' b' j' st c1 dmc1 dmc smbj c1_in_st c_in_st uniq.
-    apply (Game8_dm_m2 _ _ _ a' b' j' st c1) => //.
-    + smt(get_setE).
-    smt(get_setE).
-
-  move => a' b' i' st c1 c2 dmc1 dmc2 dmc smai' c1_in_st c2_in_st c_in_st uniq.
-  apply (Game8_dm_m3 _ _ _ a' b' i' st c1 c2) => //.
-  + smt(get_setE).
+  smt(get_setE).
+  smt(get_setE).
+  smt(get_setE).
+  smt(get_setE).
+  smt(get_setE).
+  smt(get_setE).
+  smt(get_setE).
   smt(get_setE).
 
 seq 1 : (#pre); 1: by auto.
 sp; if=> //.
 auto=> />.
-move=> &m bad dm ? inv1 inv2 inv3 inv4 ai_in_sm nbad ? ?.
-have smai : Game8.state_map.[a, i]{m} = Some (role, IPending (b, psk, na, ca) m1){m} by smt().
-case (inv1 a{m} i{m}); rewrite smai => //.
-move => /> !->> ca_in_dm ca3_nin_dm.
-have dmm2: (((a, b), msg2_data a b ca, m2) \in Game8.dec_map){m} by smt().
-case (inv2 m2{m}); 1,2,4: smt().
-move => ? ? j stb c1' _ /(inv3 _ _ _ _ _ dmm2) /> smbj ca_in_stb m2_in_stb uniq.
+move => &m _ dm sm uniq_pi uniq_pr uniq_comp ss_log_ip ss_log_rp ss_log_acc ss_log_obs sk_obs ai_in /negb_or [_ uniq] nab _.
 do! split.
 
-(* State Map invariant *)
-move => a' i'.
-case: ((a', i') = (a, i){m}) => /> => [| neq].
-+ apply (Game8_accepted_i _ _ _ _ _ b{m} j stb ca{m} m2{m} caf{m}) => //.
-  + by rewrite get_set_sameE.
-  + by rewrite mem_set.
-  + smt(get_set_neqE).
-  + case (inv1 b{m} j); rewrite smbj //.
-    + smt(get_setE).
-    + smt(get_setE).
-    + move => a'' i'' sta'' c1 c2 c3.
-      case (inv2 c3); smt().
-    + move =>  /> id1 id2 c1 c2 c3.
-      case (inv2 c3); smt().
-  smt().
-
-case (inv1 a' i').
-+ move => sm.
-  apply Game8_undef.
-  by rewrite get_set_neqE.
-+ move => sm.
-  apply (Game8_aborted_r1 _ _ _ _ _).
-  by rewrite get_set_neqE.
-+ move => b' c1 sma' dmc1.
-  apply (Game8_aborted_i _ _ _ _ _ b' c1) => //.
-  + by rewrite get_set_neqE.
-  by rewrite mem_set; left.
-+ move => b' c1 c2 sma' dmc2.
-  apply (Game8_aborted_r2 _ _ _ _ _ b' c1 c2) => //.
-  + by rewrite get_set_neqE.
-  by rewrite mem_set; left.
-+ move => b' c1 sma' dmc1 ndmc1.
-  apply (Game8_ipending _ _ _ _ _ b' c1) => //.
-  + by rewrite get_set_neqE.
-  + by rewrite mem_set; left.
-  move => c2 c3.
-  case (inv2 ca{m}); smt(mem_set).
-+ move => b' c1 c2 sma' dmc2.
-  apply (Game8_rpending _ _ _ _ _ b' c1 c2) => //.
-  + by rewrite get_set_neqE.
-  by rewrite mem_set; left.
-+ move => b' j' stb' c1 c2 c3 sma' dmc3 nsk smbj' c_in_stb' neq_bj'.
-  apply (Game8_accepted_i _ _ _ _ _ b' j' stb' c1 c2 c3) => //.
-  + by rewrite get_set_neqE.
-  + smt(get_setE).
-  smt(get_setE).
-+ move => b' j' st c1 c2 c3 sma' dmc3 smbj' obs_sk.
-  apply (Game8_accepted_r _ _ _ _ _ b' j' st c1 c2 c3) => //.
-  + by rewrite get_set_neqE.
-  + smt(get_setE).
-  smt(get_setE).
-move => r id1 id2 c1 c2 c3 k sma' dmc3 skm_k ids_eq.
-apply (Game8_observed _ _ _ _ _ r id1 id2 c1 c2 c3 k) => //.
-+ by rewrite get_set_neqE.
-by rewrite mem_set; left.
-
-(* Decmap invariant *)
-move => c.
-case (c = caf{m}) => /> => [| neq].
-+ apply (Game8_dm_m3 _ _ _ a{m} b{m} i{m} (Accepted ((a, ca), m2, caf){m} witness) ca{m} m2{m}) => //.
-  + smt(mem_set).
-  + smt(mem_set).
-  + by rewrite mem_set; right.
-  + by rewrite get_set_sameE.
-  + move => [b' j'] st'.
-    rewrite get_setE.
-    case ((b', j') = (a, i){m}) => />.
-    move => neq smbj'.
-    case (inv1 b' j'); rewrite smbj' //=.
-    + smt().
-    + smt().
-    + move => /> b c1 c2 c3.
-      case (inv2 c3); smt().
-    move => /> id1 id2 c1 c2 c3.
-    case (inv2 c3); smt().
-
-case (inv2 c).
-+ move => ndm1 ndm2 ndm3.
-  apply (Game8_dm_undef _ _ _) => //.
-  + smt(mem_set).
-  + smt(mem_set).
-  smt(mem_set).
-
-+ move => a' b' i' st.
-  case ((a', i') = (a, i){m}) => /> => [| neq'].
-  + rewrite smai => /> dmc uniq'.
-    apply (Game8_dm_m1 _ _ _ a{m} b{m} i{m} (Accepted ((a, ca), m2, caf){m} witness)) => //.
-    + smt(mem_set).
-    + by rewrite get_set_sameE.
-    smt(get_setE).
-  move => dmc smai' c_in_st uniq'.
-  apply (Game8_dm_m1 _ _ _ a' b' i' st) => //.
-  + smt(mem_set).
-  + smt(get_setE).
-  smt(get_setE).
-
-+ move => a' b' j' st c1 dmc1 dmc smbj' c1_in_st c_in_st uniq'.
-  apply (Game8_dm_m2 _ _ _ a' b' j' st c1) => //.
-  + smt(mem_set).
-  + smt(mem_set).
-  + smt(get_setE).
-  smt(get_setE).
-
-move => a' b' i' st c1 c2 dmc1 dmc2 dmc smai' c1_in_st c2_in_st c_in_st uniq'.
-apply (Game8_dm_m3 _ _ _ a' b' i' st c1 c2) => //.
-+ smt(mem_set).
-+ smt(mem_set).
-+ smt(mem_set).
-+ smt(get_setE).
-case (inv2 ca{m}); smt(get_setE).
-
-(* Ciphertext Decmap Uniqueness *)
-smt(mem_set).
-
-smt(mem_set).
+smt(get_setE).
+smt(get_setE).
+smt(get_setE).
+smt(get_setE).
+smt(get_setE).
+smt(get_setE).
+smt(get_setE).
+smt(get_setE).
 qed.
 
 hoare Game8_inv_send_fin: Game8.send_fin:
-  Game8_inv_full Game8.state_map Game8.dec_map Game8.sk_map
+  Game8_inv Game8.state_map Game8.dec_map Game8.sk_map
   ==>
-  Game8_inv_full Game8.state_map Game8.dec_map Game8.sk_map.
+  Game8_inv Game8.state_map Game8.dec_map Game8.sk_map.
 proof.
 proc.
 sp; wp ^if; if=> //.
 sp; match => //.
 sp; match => //.
 + auto=> />.
-  move=> &m ? ? inv1 inv2 inv3 inv4 ?.
-  have smbj : Game8.state_map.[b, j]{m} = Some (role, RPending (a, psk, na, nb, ca, cb) m1 m2){m} by smt().
-  case (inv1 b{m} j{m}); rewrite smbj //=.
-  move => /> !->> dmcb.
-  do! split.
-
-  (* State Map invariant *)
-  move=> b' j'.
-  case: ((b', j') = (b, j){m}) => /> => [|neq_bj].
-  - apply (Game8_aborted_r2 _ _ _ _ _ a{m} ca{m} cb{m}) => //.
-    by rewrite get_set_sameE.
-
-  case (inv1 b' j').
-  + move => sm.
-    apply Game8_undef.
-    by rewrite get_set_neqE.
-  + move => sm.
-    apply (Game8_aborted_r1 _ _ _ _ _).
-    by rewrite get_set_neqE.
-  + move => a' c1 sma' dm.
-    apply (Game8_aborted_i _ _ _ _ _ a' c1) => //.
-    by rewrite get_set_neqE.
-  + move => a' c1 c2 smb' dmc2.
-    apply (Game8_aborted_r2 _ _ _ _ _ a' c1 c2) => //.
-    by rewrite get_set_neqE.
-  + move => a' c1 smb' dmc1 ndmc1.
-    apply (Game8_ipending _ _ _ _ _ a' c1) => //.
-    by rewrite get_set_neqE.
-  + move => a' c1 c2 smb' dmc2.
-    apply (Game8_rpending _ _ _ _ _ a' c1 c2) => //.
-    by rewrite get_set_neqE.
-  + move => a' i st c1 c2 c3.
-    case ((a', i) = (b, j){m}).
-    + move => />.
-      rewrite smbj => /> smbj' dmc3 nsk ? ? ?.
-      apply (Game8_accepted_i _ _ _ _ _ b{m} j{m} (Aborted (R2 ca{m} cb{m})) c1 c2 c3) => //.
-      + by rewrite get_set_neqE.
-      smt(get_setE).
-    move => neq smbj' dmc3 nsk smai' c_in_st neq_ai.
-    apply (Game8_accepted_i _ _ _ _ _ a' i st c1 c2 c3) => //.
-    + by rewrite get_set_neqE.
-    smt(get_setE).
-  + move => a' i st c1 c2 c3 smb' dmc3 smai obs_sk.
-    apply (Game8_accepted_r _ _ _ _ _ a' i st c1 c2 c3) => //.
-    + by rewrite get_set_neqE.
-    smt(get_set_neqE).
-  move => r id1 id2 c1 c2 c3 k smb' dmc3 skm_k ids_eq.
-  apply (Game8_observed _ _ _ _ _ r id1 id2 c1 c2 c3 k) => //.
-  by rewrite get_set_neqE.
-
-  (* Decmap invariant *)
-  move => c.
-
-  case (inv2 c).
-  + move => ndm1 ndm2 ndm3.
-    exact (Game8_dm_undef _ _ _).
-
-  + move => a' b' i' st dmc smai c_in_st uniq.
-    apply (Game8_dm_m1 _ _ _ a' b' i' st) => //.
-    + smt(get_setE).
-    smt(get_setE).
-
-  + move => a' b' j' st c1.
-    case ((b', j') = (b, j){m}) => /> => [| neq].
-    + rewrite smbj => /> dmc1 dmc c1_eqs c_eqs uniq.
-      apply (Game8_dm_m2 _ _ _ a{m} b{m} j{m} (Aborted (R2 ca{m} cb{m})) ca{m}) => //.
-      + smt().
-      + smt().
-      + by rewrite get_set_sameE.
-      smt(get_setE).
-    move => dmc1 dmc smbj' c1_in_st c_in_st uniq.
-    apply (Game8_dm_m2 _ _ _ a' b' j' st c1) => //.
-    + smt(get_setE).
-    smt(get_setE).
-
-  move => a' b' i' st c1 c2 dmc1 dmc2 dmc smai c1_in_st c2_in_st c_in_st uniq.
-  apply (Game8_dm_m3 _ _ _ a' b' i' st c1 c2) => //.
-  + smt(get_setE).
   smt(get_setE).
-
-auto=> />.
-move=> &m ? ? inv1 inv2 inv3 inv4 bjin.
-have smbj : Game8.state_map.[b, j]{m} = Some (role, RPending (a, psk, na, nb, ca, cb) m1 m2){m} by smt().
-case (inv1 b{m} j{m}); rewrite smbj //=.
-move => /> !->> dmcb.
-have dmm3: (((a, b), msg3_data a b ca cb, m3) \in Game8.dec_map){m} by smt().
-case (inv2 m3{m}); 1..3: smt().
-move => a' b' i sta c1 c2 dmca _ /(inv3 _ _ _ _ _ dmm3) /> smai ca_in_sta cb_in_sta m3_in_sta uniq.
-clear a' b' c1 c2.
+auto => />.
+move => &m dm sm uniq_pi uniq_pr uniq_comp ss_log_ip ss_log_rp ss_log_acc ss_log_obs sk_obs ai_in.
 do! split.
 
-(* State Map invariant *)
-move=> b' j'.
-case: ((b', j') = (b, j){m}) => /> => [|neq_bj].
-- apply (Game8_accepted_r _ _ _ _ _ a{m} i sta ca{m} cb{m} m3{m}) => //.
-  + smt(get_setE).
-  + smt(get_setE).
-  + by case: (inv1 a{m} i); rewrite smai=> // /#.
-  + case (inv1 a{m} i); rewrite smai=> // />.
-    + smt().
-    + smt().
-    by case (inv2 cb{m})=> /#.
-
-case (inv1 b' j').
-+ move => sm.
-  apply Game8_undef.
-  by rewrite get_set_neqE.
-+ move => sm.
-  apply (Game8_aborted_r1 _ _ _ _ _).
-  by rewrite get_set_neqE.
-+ move => a' c1 sma' dm.
-  apply (Game8_aborted_i _ _ _ _ _ a' c1) => //.
-  by rewrite get_set_neqE.
-+ move => a' c1 c2 smb' dmc2.
-  apply (Game8_aborted_r2 _ _ _ _ _ a' c1 c2) => //.
-  by rewrite get_set_neqE.
-+ move => a' c1 smb' dmc1 ndmc1.
-  apply (Game8_ipending _ _ _ _ _ a' c1) => //.
-  by rewrite get_set_neqE.
-+ move => a' c1 c2 smb' dmc2.
-  apply (Game8_rpending _ _ _ _ _ a' c1 c2) => //.
-  by rewrite get_set_neqE.
-+ move => b'' j'' st c1 c2 c3.
-  case ((b'', j'') = (b, j){m}).
-  + move => />.
-    rewrite smbj => /> smbj' dmc3 nsk ? ? ?.
-    apply (Game8_accepted_i _ _ _ _ _ b{m} j{m} (Accepted ((a, ca), cb, m3) witness){m} c1 c2 c3) => //.
-    + by rewrite get_set_neqE.
-    + by rewrite get_set_sameE.
-    + smt().
-    case (inv2 ca{m}); 1,3,4: smt().
-    move => a'' b''' i' sta'' /(inv3 _ _ _ _ _ dmca) [] [] /= <*> /=.
-    move => _ _ uniq'.
-    clear sta''.
-    case (inv2 c3) => /#.
-  move => neq sma' dmc3 nsk smai' c_in_st neq'.
-  apply (Game8_accepted_i _ _ _ _ _ b'' j'' st c1 c2 c3) => //.
-  + by rewrite get_set_neqE.
-  smt(get_set_neqE).
-+ move => a' i' st c1 c2 c3 smb' dmc3 smai' obs_sk.
-  apply (Game8_accepted_r _ _ _ _ _ a' i' st c1 c2 c3) => //.
-  + by rewrite get_set_neqE.
-  smt(get_set_neqE).
-move => r id1 id2 c1 c2 c3 k smb' dmc3 skm_k ids_eq.
-apply (Game8_observed _ _ _ _ _ r id1 id2 c1 c2 c3 k) => //.
-by rewrite get_set_neqE.
-
-(* Decmap invariant *)
-move => c.
-
-case (inv2 c).
-+ move => ndm1 ndm2 ndm3.
-  exact (Game8_dm_undef _ _ _).
-
-+ move => a' b' i' st dmc smai' c_in_st uniq'.
-  apply (Game8_dm_m1 _ _ _ a' b' i' st) => //.
-  + smt(get_setE).
-  smt(get_setE).
-
-+ move => a' b' j' st c1.
-  case ((b', j') = (b, j){m}) => /> => [| neq].
-  + rewrite smbj => /> dmc1 dmc c1_eqs c_eqs uniq'.
-    apply (Game8_dm_m2 _ _ _ a{m} b{m} j{m} (Accepted ((a, ca), cb, m3){m} witness) ca{m}) => //.
-    + smt().
-    + by rewrite get_set_sameE.
-    smt(get_setE).
-    smt(get_setE).
-  move => dmc1 dmc smbj' c1_in_st c_in_st uniq'.
-  apply (Game8_dm_m2 _ _ _ a' b' j' st c1) => //.
-  + smt(get_setE).
-  smt(get_setE).
-
-move => a' b' i' st c1 c2 dmc1 dmc2 dmc smai' c1_in_st c2_in_st c_in_st uniq'.
-apply (Game8_dm_m3 _ _ _ a' b' i' st c1 c2) => //.
-+ smt(get_setE).
+smt(get_setE).
+smt(get_setE).
+smt(get_setE).
+smt(get_setE).
+smt(get_setE).
+move => v x r b' m1' m2' m3' sk.
+rewrite get_setE.
+case ((v, x) = (b, j){m}).
++ smt().
+smt().
+smt(get_setE).
 smt(get_setE).
 qed.
 
 hoare Game8_inv_reveal: Game8.reveal:
-  Game8_inv_full Game8.state_map Game8.dec_map Game8.sk_map
+  Game8_inv Game8.state_map Game8.dec_map Game8.sk_map
   ==>
-  Game8_inv_full Game8.state_map Game8.dec_map Game8.sk_map.
+  Game8_inv Game8.state_map Game8.dec_map Game8.sk_map.
 proof.
 proc.
 sp; wp ^if; if => //.
 sp; match; 1,2,4,5: by auto.
 sp; if => //.
 rcondt ^if.
-+ auto => /> &m st inv1 inv2 inv3 inv4 aiin card_obs_ps sk _.
-  have smai : Game8.state_map.[a, i]{m} = Some (role{m}, Accepted trace{m} k'{m}) by smt().
-  case (inv1 a{m} i{m}); rewrite smai //.
-  + move => />.
-    move => b j stb c1 c2 c3 !->> dmc3 smbj.
-    case (inv1 b j); rewrite smbj //.
-    move => />.
-    move => id1 id2 c1' c2' c3' k'.
-    move => ->>.
-    case (inv2 c3'); 1..3: smt().
-    case (c1' = c1); 2: smt().
-    case (c2' = c2); 2: smt().
-    case (c3' = c3); 2: smt().
-    case (id1 = a{m}); 2: smt().
-    move => />.
-    have bj_partner : (b, j) \in get_partners (Some ((a{m}, c1), c2, c3)) Initiator Game8.state_map{m}.
-    + rewrite /get_partners mem_fdom mem_filter /#.
-    have // : (b, j) \in get_observed_partners (a, i){m} Game8.state_map{m}.
-    + rewrite /get_observed_partners in_filter /#.
-    rewrite fcard_eq0 in card_obs_ps.
-    by rewrite card_obs_ps in_fset0.
-  move => />.
-  move => b j stb c1 c2 c3 !->> dmc3 smbj.
-  case (inv1 b j); rewrite smbj //.
-  move => />.
-  move => id1 id2 c1' c2' c3' k'.
-  move => ->>.
-  case (inv2 c3'); 1..3: smt().
-  case (c1' = c1); 2: smt().
-  case (c2' = c2); 2: smt().
-  case (c3' = c3); 2: smt().
-  case (id1 = b); 2: smt().
-  move => />.
-  have bj_partner : (b, j) \in get_partners (Some ((b, c1), c2, c3)) Responder Game8.state_map{m}.
++ auto => />.
+  move => &m smai uniq_pi uniq_pr uniq_comp ss_log_ip ss_log_rp ss_log_acc ss_log_obs sk_obs ai_in obs_ps k _.
+  case (trace{m} \in Game8.sk_map{m}) => // ^ tr_in_skm.
+  move => /(sk_obs trace{m}) [a' i' r sk smai'].
+  have := uniq_comp trace{m} (a, i){m} (a', i') role{m} (Accepted trace{m} k'{m}) (Observed trace{m} sk).
+  have -> : Game8.state_map{m}.[a{m}, i{m}] = Some (role{m}, Accepted trace{m} k'{m}) by smt().
+  rewrite smai' some_oget //=.
+  case (r = role{m}) => //.
+  move => neq_role.
+  have bj_partner : (a', i') \in get_partners (Some trace{m}) role{m} Game8.state_map{m}.
   + rewrite /get_partners mem_fdom mem_filter /#.
-  have // : (b, j) \in get_observed_partners (a, i){m} Game8.state_map{m}.
+  have // : (a', i') \in get_observed_partners (a, i){m} Game8.state_map{m}.
   + rewrite /get_observed_partners in_filter /#.
-  rewrite fcard_eq0 in card_obs_ps.
-  by rewrite card_obs_ps in_fset0.
+  rewrite fcard_eq0 in obs_ps.
+  by rewrite obs_ps in_fset0.
 
-auto => /> &m st inv1 inv2 inv3 inv4 aiin card_obs_ps sk _.
-rewrite get_set_sameE //=.
-
-case: (role{m}) aiin st => /> /domE; case _: (Game8.state_map.[a, i]{m})=> /> smai.
-case (inv1 a{m} i{m}); rewrite smai=> //=.
-move => /> b j stb c1 c2 c3 !->> dmc3 smbj c1_in_stb c2_in_stb c3_in_stb nskm.
+auto => />.
+move => &m smai uniq_pi uniq_pr uniq_comp ss_log_ip ss_log_rp ss_log_acc ss_log_obs sk_obs ai_in obs_ps k _.
 do! split.
 
-(* State Map invariant *)
-move=> a' i'.
-case: ((a', i') = (a, i){m}) => /> => [|neq_ai].
-- apply (Game8_observed _ _ _ _ _ Initiator a{m} b c1 c2 c3 sk) => //.
-  + by rewrite get_set_sameE.
-  by rewrite mem_set; right.
-
-case (inv1 a' i').
-+ move => sm.
-  apply Game8_undef.
-  by rewrite get_set_neqE.
-+ move => sm.
-  apply (Game8_aborted_r1 _ _ _ _ _).
-  by rewrite get_set_neqE.
-+ move => b' c1' smb' dm.
-  apply (Game8_aborted_i _ _ _ _ _ b' c1') => //.
-  by rewrite get_set_neqE.
-+ move => b' c1' c2' sma' dmc2.
-  apply (Game8_aborted_r2 _ _ _ _ _ b' c1' c2') => //.
-  by rewrite get_set_neqE.
-+ move => b' c1' sma' dmc1 ndmc1.
-  apply (Game8_ipending _ _ _ _ _ b' c1') => //.
-  by rewrite get_set_neqE.
-+ move => b' c1' c2' sma' dmc2.
-  apply (Game8_rpending _ _ _ _ _ b' c1' c2') => //.
-  by rewrite get_set_neqE.
-+ move => b' j' stb' c1' c2' c3' sma' dmc3' smbj' c_in_stb' c3'_tr obs_sk.
-  apply (Game8_accepted_i _ _ _ _ _ b' j' stb' c1' c2' c3') => //.
-  + by rewrite get_set_neqE.
-  + smt(get_setE).
-  + case (inv2 c3); smt(get_setE).
-+ move => b'' j' stb' c1' c2' c3'.
-  case ((b'', j') = (a, i){m}).
-  + move => />.
-    rewrite smai => /> smai' dmc3'.
-    case (inv2 c3'); 1..3: smt().
-    move => />.
-    have /> := inv3 _ _ _ _ _ dmc3 dmc3'.
-    move => *.
-    apply (Game8_accepted_r _ _ _ _ _ a{m} i{m} (Observed ((a{m}, c1'), c2', c3') sk) c1' c2' c3') => //.
-    + smt(get_setE).
-    by rewrite get_set_sameE.
-  move => neqbj' sma' dmc3' smbj' c_in_stb obs_skmn.
-  apply (Game8_accepted_r _ _ _ _ _ b'' j' stb' c1' c2' c3') => //.
-  + by rewrite get_set_neqE.
-  + smt(get_setE).
-  by case (inv2 c3); smt(get_setE).
-move => r id1 id2 c1' c2' c3' k smb' dmc3' skm_k ids_eq.
-apply (Game8_observed _ _ _ _ _ r id1 id2 c1' c2' c3' k) => //.
-+ by rewrite get_set_neqE.
-+ rewrite mem_set; left.
-exact skm_k.
-
-(* Decmap invariant *)
-move => c.
-
-case (inv2 c).
-+ move => ndm1 ndm2 ndm3.
-  exact (Game8_dm_undef _ _ _).
-
-+ move => a' b' i'.
-  case ((a', i') = (a, i){m}) => />.
-  + rewrite smai => />.
-    move => dmc eq_c uniq.
-    apply (Game8_dm_m1 _ _ _ a{m} b' i{m} (Observed ((a{m}, c1), c2, c3) sk)) => //.
-    + by rewrite get_set_sameE.
-    smt(get_setE).
-  move => neq st' dmc smai' c_in_st uniq.
-  apply (Game8_dm_m1 _ _ _ a' b' i' st') => //.
-  + by rewrite get_set_neqE.
-  smt(get_setE).
-
-+ move => a' b' j' st' c1' dmc1' dmc smbj' c1_in_st c_in_st uniq.
-  apply (Game8_dm_m2 _ _ _ a' b' j' st' c1') => //.
-  + smt(get_setE).
-  smt(get_setE).
-
-move => a' b' i'.
-case ((a', i') = (a, i){m}) => />.
-+ rewrite smai => />.
-  move => c1' c2' dmc1' dmc2' dmc smai' c1_in_st c2_in_st uniq.
-  apply (Game8_dm_m3 _ _ _ a{m} b' i{m} (Observed ((a{m}, c1), c2, c3) sk) c1 c2) => //.
-  + smt(mem_set).
-  + smt(mem_set).
-  + smt(mem_set).
-  + smt(get_setE).
-  smt(get_setE).
-move => neq st' c1' c2' dmc1' dmc2' dmc smai' c1_in_st c2_in_st c_in_st uniq.
-apply (Game8_dm_m3 _ _ _ a' b' i' st' c1' c2') => //.
-+ smt(get_setE).
 smt(get_setE).
-
 smt(get_setE).
-
-case (inv1 a{m} i{m}); rewrite smai //=.
-move => /> b j stbj c1 c2 c3 !->> dmc3 smbj trace_stbj obs_skm.
-do! split.
-
-(* State Map invariant *)
-move=> a' i'.
-case: ((a', i') = (a, i){m}) => /> => [|neq_ai].
-- apply (Game8_observed _ _ _ _ _ Responder b a{m} c1 c2 c3 sk) => //.
-  + by rewrite get_set_sameE.
-  by rewrite mem_set; right.
-
-case (inv1 a' i').
-+ move => sm.
-  apply Game8_undef.
-  by rewrite get_set_neqE.
-+ move => sm.
-  apply (Game8_aborted_r1 _ _ _ _ _).
-  by rewrite get_set_neqE.
-+ move => b' c1' smb' dm.
-  apply (Game8_aborted_i _ _ _ _ _ b' c1') => //.
-  by rewrite get_set_neqE.
-+ move => b' c1' c2' sma' dmc2.
-  apply (Game8_aborted_r2 _ _ _ _ _ b' c1' c2') => //.
-  by rewrite get_set_neqE.
-+ move => b' c1' sma' dmc1 ndmc1.
-  apply (Game8_ipending _ _ _ _ _ b' c1') => //.
-  by rewrite get_set_neqE.
-+ move => b' c1' c2' sma' dmc2.
-  apply (Game8_rpending _ _ _ _ _ b' c1' c2') => //.
-  by rewrite get_set_neqE.
-+ move => b' j' stb' c1' c2' c3'.
-  case ((b', j') = (a, i){m}).
-  + move => />.
-    rewrite smai => /> *.
-    apply (Game8_accepted_i _ _ _ _ _ a{m} i{m} (Observed ((b, c1), c2, c3) sk) c1' c2' c3') => //.
-    + by rewrite get_set_neqE.
-    + by rewrite get_set_sameE.
-  move => neq' smai' dmc3' smbj' c_in_stb' c3'_tr obs_sk.
-  apply (Game8_accepted_i _ _ _ _ _ b' j' stb' c1' c2' c3') => //.
-  + by rewrite get_set_neqE.
-  + smt(get_setE).
-  move => ^ /obs_sk.
-  rewrite mem_set negb_or //=.
-  case (c3' = c3); 2: smt().
-  case (c2' = c2); 2: smt().
-  case (c1' = c1); 2: smt().
-  move => />.
-  case (inv2 c3); 1..3: smt().
-  case (inv2 c2); 1,2,4: smt().
-  smt().
-+ move => b' j' stb c1' c2' c3' sma' dmc3' smbj' c_in_stb obs_sk.
-  apply (Game8_accepted_r _ _ _ _ _ b' j' stb c1' c2' c3') => //.
-  + by rewrite get_set_neqE.
-  + smt(get_setE).
-  case (inv2 c3); 1..3: smt().
-  case (inv2 c2); 1,2,4: smt().
-  smt(mem_set).
-move => r id1 id2 c1' c2' c3' k smb' dmc3' skm_k ids_eq.
-apply (Game8_observed _ _ _ _ _ r id1 id2 c1' c2' c3' k) => //.
-+ by rewrite get_set_neqE.
-+ rewrite mem_set; left.
-exact skm_k.
-
-(* Decmap invariant *)
-move => c.
-
-case (inv2 c).
-+ move => ndm1 ndm2 ndm3.
-  exact (Game8_dm_undef _ _ _).
-
-+ move => a' b' i' st' dmc smai' c_in_st' uniq.
-  apply (Game8_dm_m1 _ _ _ a' b' i' st') => //.
-  + smt(get_setE).
-  smt(get_setE).
-
-+ move => a' b' j' st' c1'.
-  case ((b', j') = (a, i){m}).
-  + move => /> *.
-    apply (Game8_dm_m2 _ _ _ a' a{m} i{m} (Observed ((b, c1), c2, c3) sk) c1') => //.
-    + smt(get_setE).
-    + smt(get_setE).
-    + smt(get_setE).
-    smt(get_setE).
-  move => neq' dmc1' dmc smbj' c1_in_st c_in_st uniq.
-  apply (Game8_dm_m2 _ _ _ a' b' j' st' c1') => //.
-  + smt(get_setE).
-  smt(get_setE).
-
-move => a' b' i'.
-move => st' c1' c2' dmc1' dmc2' dmc smai' c1_in_st c2_in_st c_in_st uniq.
-apply (Game8_dm_m3 _ _ _ a' b' i' st' c1' c2') => //.
-+ smt(get_setE).
 smt(get_setE).
-
+smt(get_setE).
+smt(get_setE).
+smt(get_setE).
+smt(get_setE).
 smt(get_setE).
 qed.
 
 hoare Game8_inv_test: Game8.test:
-  Game8_inv_full Game8.state_map Game8.dec_map Game8.sk_map
+  Game8_inv Game8.state_map Game8.dec_map Game8.sk_map
   ==>
-  Game8_inv_full Game8.state_map Game8.dec_map Game8.sk_map.
+  Game8_inv Game8.state_map Game8.dec_map Game8.sk_map.
 proof.
 proc.
 sp; wp ^if; if => //.
 sp; match; 1,2,4,5: by auto.
 sp; if => //.
 rcondt ^if.
-+ auto => /> &m st inv1 inv2 inv3 inv4 aiin card_obs_ps sk _.
-  have smai : Game8.state_map.[a, i]{m} = Some (role{m}, Accepted trace{m} k'{m}) by smt().
-  case (inv1 a{m} i{m}); rewrite smai //.
-  + move => />.
-    move => b j stb c1 c2 c3 !->> dmc3 smbj.
-    case (inv1 b j); rewrite smbj //.
-    move => />.
-    move => id1 id2 c1' c2' c3' k'.
-    move => ->>.
-    case (inv2 c3'); 1..3: smt().
-    case (c1' = c1); 2: smt().
-    case (c2' = c2); 2: smt().
-    case (c3' = c3); 2: smt().
-    case (id1 = a{m}); 2: smt().
-    move => />.
-    have bj_partner : (b, j) \in get_partners (Some ((a{m}, c1), c2, c3)) Initiator Game8.state_map{m}.
-    + rewrite /get_partners mem_fdom mem_filter /#.
-    have // : (b, j) \in get_observed_partners (a, i){m} Game8.state_map{m}.
-    + rewrite /get_observed_partners in_filter /#.
-    rewrite fcard_eq0 in card_obs_ps.
-    by rewrite card_obs_ps in_fset0.
-  move => />.
-  move => b j stb c1 c2 c3 !->> dmc3 smbj.
-  case (inv1 b j); rewrite smbj //.
-  move => />.
-  move => id1 id2 c1' c2' c3' k'.
-  move => ->>.
-  case (inv2 c3'); 1..3: smt().
-  case (c1' = c1); 2: smt().
-  case (c2' = c2); 2: smt().
-  case (c3' = c3); 2: smt().
-  case (id1 = b); 2: smt().
-  move => />.
-  have bj_partner : (b, j) \in get_partners (Some ((b, c1), c2, c3)) Responder Game8.state_map{m}.
++ auto => />.
+  move => &m smai uniq_pi uniq_pr uniq_comp ss_log_ip ss_log_rp ss_log_acc ss_log_obs sk_obs ai_in obs_ps k _.
+  case (trace{m} \in Game8.sk_map{m}) => // ^ tr_in_skm.
+  move => /(sk_obs trace{m}) [a' i' r sk smai'].
+  have := uniq_comp trace{m} (a, i){m} (a', i') role{m} (Accepted trace{m} k'{m}) (Observed trace{m} sk).
+  have -> : Game8.state_map{m}.[a{m}, i{m}] = Some (role{m}, Accepted trace{m} k'{m}) by smt().
+  rewrite smai' some_oget //=.
+  case (r = role{m}) => //.
+  move => neq_role.
+  have bj_partner : (a', i') \in get_partners (Some trace{m}) role{m} Game8.state_map{m}.
   + rewrite /get_partners mem_fdom mem_filter /#.
-  have // : (b, j) \in get_observed_partners (a, i){m} Game8.state_map{m}.
+  have // : (a', i') \in get_observed_partners (a, i){m} Game8.state_map{m}.
   + rewrite /get_observed_partners in_filter /#.
-  rewrite fcard_eq0 in card_obs_ps.
-  by rewrite card_obs_ps in_fset0.
+  rewrite fcard_eq0 in obs_ps.
+  by rewrite obs_ps in_fset0.
 
 seq 1 : #pre; 1: by auto => />.
 sp.
-seq 1 : #pre; 1: by auto => />.
-
-auto => /> &m skm st inv1 inv2 inv3 inv4 aiin card_obs_ps.
-
-case: (role{m}) aiin st => /> /domE; case _: (Game8.state_map.[a, i]{m})=> /> smai.
-case (inv1 a{m} i{m}); rewrite smai //=.
-move => /> b j stb c1 c2 c3 !->> dmc3 smbj c1_in_stb c2_in_stb c3_in_stb nskm.
-do! split.
-
-(* State Map invariant *)
-move=> a' i'.
-case: ((a', i') = (a, i){m}) => /> => [|neq_ai].
-- apply (Game8_observed _ _ _ _ _ Initiator a{m} b c1 c2 c3 k{m}) => //.
-  + by rewrite get_set_sameE.
-  by rewrite mem_set; right.
-
-case (inv1 a' i').
-+ move => sm.
-  apply Game8_undef.
-  by rewrite get_set_neqE.
-+ move => sm.
-  apply (Game8_aborted_r1 _ _ _ _ _).
-  by rewrite get_set_neqE.
-+ move => b' c1' smb' dm.
-  apply (Game8_aborted_i _ _ _ _ _ b' c1') => //.
-  by rewrite get_set_neqE.
-+ move => b' c1' c2' sma' dmc2.
-  apply (Game8_aborted_r2 _ _ _ _ _ b' c1' c2') => //.
-  by rewrite get_set_neqE.
-+ move => b' c1' sma' dmc1 ndmc1.
-  apply (Game8_ipending _ _ _ _ _ b' c1') => //.
-  by rewrite get_set_neqE.
-+ move => b' c1' c2' sma' dmc2.
-  apply (Game8_rpending _ _ _ _ _ b' c1' c2') => //.
-  by rewrite get_set_neqE.
-+ move => b' j' stb' c1' c2' c3' sma' dmc3' smbj' c_in_stb' c3'_tr obs_sk.
-  apply (Game8_accepted_i _ _ _ _ _ b' j' stb' c1' c2' c3') => //.
-  + by rewrite get_set_neqE.
-  + smt(get_setE).
-  + by case (inv2 c3'); smt(get_setE).
-+ move => b'' j' stb' c1' c2' c3'.
-  case ((b'', j') = (a, i){m}).
-  + move => />.
-    rewrite smai => /> smai' dmc3'.
-    case (inv2 c3'); 1..3: smt(get_setE).
-    move => />.
-    have /> := inv3 _ _ _ _ _ dmc3 dmc3'.
-    move => *.
-    apply (Game8_accepted_r _ _ _ _ _ a{m} i{m} (Observed ((a{m}, c1'), c2', c3') k{m}) c1' c2' c3') => //.
-    + smt(get_setE).
-    by rewrite get_set_sameE.
-  move => neqbj' sma' dmc3' smbj' c_in_stb obs_skmn.
-  apply (Game8_accepted_r _ _ _ _ _ b'' j' stb' c1' c2' c3') => //.
-  + by rewrite get_set_neqE.
-  + smt(get_setE).
-  by case (inv2 c3'); smt(get_setE).
-move => r id1 id2 c1' c2' c3' k smb' dmc3' skm_k ids_eq.
-apply (Game8_observed _ _ _ _ _ r id1 id2 c1' c2' c3' k) => //.
-+ by rewrite get_set_neqE.
-+ rewrite mem_set; left.
-exact skm_k.
-
-(* Decmap invariant *)
-move => c.
-
-case (inv2 c).
-+ move => ndm1 ndm2 ndm3.
-  exact (Game8_dm_undef _ _ _).
-
-+ move => a' b' i'.
-  case ((a', i') = (a, i){m}) => />.
-  + rewrite smai => />.
-    move => dmc eq_c uniq.
-    apply (Game8_dm_m1 _ _ _ a{m} b' i{m} (Observed ((a{m}, c1), c2, c3) k{m})) => //.
-    + by rewrite get_set_sameE.
-    smt(get_setE).
-  move => neq st' dmc smai' c_in_st uniq.
-  apply (Game8_dm_m1 _ _ _ a' b' i' st') => //.
-  + by rewrite get_set_neqE.
+if.
++ auto => />.
+  move => &m sm smai uniq_pi uniq_pr uniq_comp ss_log_ip ss_log_rp ss_log_acc ss_log_obs sk_obs ai_in obs_ps.
+  do! split.
+  
+  smt(get_setE).
+  smt(get_setE).
+  smt(get_setE).
+  smt(get_setE).
+  smt(get_setE).
+  smt(get_setE).
+  smt(get_setE).
+  smt(get_setE).
++ auto => />.
+  move => &m sm smai uniq_pi uniq_pr uniq_comp ss_log_ip ss_log_rp ss_log_acc ss_log_obs sk_obs ai_in obs_ps _ k _.
+  do! split.
+  
+  smt(get_setE).
+  smt(get_setE).
+  smt(get_setE).
+  smt(get_setE).
+  smt(get_setE).
+  smt(get_setE).
   smt(get_setE).
 
-+ move => a' b' j' st' c1' dmc1' dmc smbj' c1_in_st c_in_st uniq.
-  apply (Game8_dm_m2 _ _ _ a' b' j' st' c1') => //.
-  + smt(get_setE).
-  smt(get_setE).
-
-move => a' b' i'.
-case ((a', i') = (a, i){m}) => />.
-+ rewrite smai => />.
-  move => c1' c2' dmc1' dmc2' dmc smai' c1_in_st c2_in_st uniq.
-  apply (Game8_dm_m3 _ _ _ a{m} b' i{m} (Observed ((a{m}, c1), c2, c3) k{m}) c1 c2) => //.
-  + smt(mem_set).
-  + smt(mem_set).
-  + smt(mem_set).
-  + smt(get_setE).
-  smt(get_setE).
-move => neq st' c1' c2' dmc1' dmc2' dmc smai' c1_in_st c2_in_st c_in_st uniq.
-apply (Game8_dm_m3 _ _ _ a' b' i' st' c1' c2') => //.
-+ smt(get_setE).
-smt(get_setE).
-
-smt(get_setE).
-
-case (inv1 a{m} i{m}); rewrite smai //=.
-move => /> b j stbj c1 c2 c3 !->> dmc3 smbj trace_stbj obs_skm.
-do! split.
-
-(* State Map invariant *)
-move=> a' i'.
-case: ((a', i') = (a, i){m}) => /> => [|neq_ai].
-- apply (Game8_observed _ _ _ _ _ Responder b a{m} c1 c2 c3 k{m}) => //.
-  + by rewrite get_set_sameE.
-  by rewrite mem_set; right.
-
-case (inv1 a' i').
-+ move => sm.
-  apply Game8_undef.
-  by rewrite get_set_neqE.
-+ move => sm.
-  apply (Game8_aborted_r1 _ _ _ _ _).
-  by rewrite get_set_neqE.
-+ move => b' c1' smb' dm.
-  apply (Game8_aborted_i _ _ _ _ _ b' c1') => //.
-  by rewrite get_set_neqE.
-+ move => b' c1' c2' sma' dmc2.
-  apply (Game8_aborted_r2 _ _ _ _ _ b' c1' c2') => //.
-  by rewrite get_set_neqE.
-+ move => b' c1' sma' dmc1 ndmc1.
-  apply (Game8_ipending _ _ _ _ _ b' c1') => //.
-  by rewrite get_set_neqE.
-+ move => b' c1' c2' sma' dmc2.
-  apply (Game8_rpending _ _ _ _ _ b' c1' c2') => //.
-  by rewrite get_set_neqE.
-+ move => b' j' stb' c1' c2' c3'.
-  case ((b', j') = (a, i){m}).
-  + move => />.
-    rewrite smai => /> *.
-    apply (Game8_accepted_i _ _ _ _ _ a{m} i{m} (Observed ((b, c1), c2, c3) k{m}) c1' c2' c3') => //.
-    + by rewrite get_set_neqE.
-    + by rewrite get_set_sameE.
-  move => neq' smai' dmc3' smbj' c_in_stb' c3'_tr obs_sk.
-  apply (Game8_accepted_i _ _ _ _ _ b' j' stb' c1' c2' c3') => //.
-  + by rewrite get_set_neqE.
-  + smt(get_setE).
-  move => ^ /obs_sk.
-  rewrite mem_set negb_or //=.
-  case (c3' = c3); 2: smt().
-  case (c2' = c2); 2: smt().
-  case (c1' = c1); 2: smt().
-  move => />.
-  case (inv2 c3); 1..3: smt().
-  case (inv2 c2); 1,2,4: smt().
-  smt().
-+ move => b' j' stb c1' c2' c3' sma' dmc3' smbj' c_in_stb obs_sk.
-  apply (Game8_accepted_r _ _ _ _ _ b' j' stb c1' c2' c3') => //.
-  + by rewrite get_set_neqE.
-  + smt(get_setE).
-  case (inv2 c3); 1..3: smt().
-  case (inv2 c2); 1,2,4: smt().
-  smt(mem_set).
-move => r id1 id2 c1' c2' c3' k smb' dmc3' skm_k ids_eq.
-apply (Game8_observed _ _ _ _ _ r id1 id2 c1' c2' c3' k) => //.
-+ by rewrite get_set_neqE.
-+ rewrite mem_set; left.
-exact skm_k.
-
-(* Decmap invariant *)
-move => c.
-
-case (inv2 c).
-+ move => ndm1 ndm2 ndm3.
-  exact (Game8_dm_undef _ _ _).
-
-+ move => a' b' i' st' dmc smai' c_in_st' uniq.
-  apply (Game8_dm_m1 _ _ _ a' b' i' st') => //.
-  + smt(get_setE).
-  smt(get_setE).
-
-+ move => a' b' j' st' c1'.
-  case ((b', j') = (a, i){m}).
-  + move => /> *.
-    apply (Game8_dm_m2 _ _ _ a' a{m} i{m} (Observed ((b, c1), c2, c3) k{m}) c1') => //.
-    + smt(get_setE).
-    + smt(get_setE).
-    + smt(get_setE).
-    smt(get_setE).
-  move => neq' dmc1' dmc smbj' c1_in_st c_in_st uniq.
-  apply (Game8_dm_m2 _ _ _ a' b' j' st' c1') => //.
-  + smt(get_setE).
-  smt(get_setE).
-
-move => a' b' i'.
-move => st' c1' c2' dmc1' dmc2' dmc smai' c1_in_st c2_in_st c_in_st uniq.
-apply (Game8_dm_m3 _ _ _ a' b' i' st' c1' c2') => //.
-+ smt(get_setE).
-smt(get_setE).
-
-smt(get_setE).
+move => t.
+rewrite mem_set.
+case; smt(get_setE).
 qed.
